wip on hash specs

providers/evercrypt/EverCrypt.Hash.fsti
@@ -3,6 +3,188 @@ module EverCrypt.Hash
 open EverCrypt.Helpers
 open FStar.HyperStack.ST
 open FStar.Integers
+ 
+/// ----------agile interface to hash specifications ----------------
+/// inlined here since EverCrypt.Hash.fst needs access to
+/// the specification implementation
+///
+
+/// Agile specification of all supported hash algorithmms.
+
+//open FStar.UInt32
+let bytes = Seq.seq UInt8.t
+type lbytes (l:nat) = b:bytes{ Seq.length b = l }
+
+/// SUPPORTED ALGORITHMS see e.g. https://en.wikipedia.org/wiki/SHA-1
+/// for a global comparison and lengths
+///
+/// * SHA224 and SHA512 are not yet multiplexed.
+/// * MD5 and SHA1 are still required by TLS 1.2, included for legacy
+///   purpose only, and not provided by HACL*.
+/// * SHA3 will be provided by HACL*.
+   
+type alg =
+  | MD5
+  | SHA1
+  | SHA224 
+  | SHA256
+  | SHA384
+  | SHA512
+//| SHAKE128 of (n:nat{n >= 8})
+//| SHAKE256 of (n:nat{n >= 16})
+
+val string_of_alg: alg -> string 
+
+
+/// HMAC/HKDF ALGORITHMS; secure_api makes security assumptions only
+/// for constructions based on those.
+/// 
+//type alg13 = a:alg {a=SHA256 \/ a=SHA384 \/ a=SHA512}
+type alg13 = alg
+type e_alg = Ghost.erased alg
+
+
+/// Lengths for input blocks and output tags, in bytes.
+
+let blockLen = function
+  | MD5 | SHA1 | SHA224 | SHA256 ->  64ul
+  | SHA384 | SHA512              -> 128ul
+//| SHAKE128 _ -> 168 | SHAKE256 _ -> 136
+  
+noextract 
+let blockLength (a: e_alg) = v (blockLen (Ghost.reveal a))
+
+let maxTagLen = 64ul
+let tagLen (a:alg) : Tot UInt32.t =
+  match a with
+  | MD5    -> 16ul
+  | SHA1   -> 20ul
+  | SHA224 -> 28ul // truncated SHA256
+  | SHA256 -> 32ul
+  | SHA384 -> 48ul // truncated SHA512
+  | SHA512 -> 64ul
+noextract 
+let tagLength a = v (tagLen (Ghost.reveal a))
+let lemma_maxLen (a:alg) = assert_norm(tagLen a <= maxTagLen)
+
+/// Maximal input lengths (from hacl*); this is overly restrictive.
+
+noextract let maxLength: e_alg -> nat = fun a -> pow2 61 - 1 
+noextract let lemma_maxLength (a: e_alg) = assert_norm (pow2 32 <= maxLength a) 
+noextract let hashable (a: e_alg) = b: bytes{ Seq.length b <= maxLength a }
+//TODO in hacl* this was enforced more concretely using the counter.
+
+/// To specify their low-level incremental computations, we assume
+/// Merkle-Damgard/sponge-like algorithms:
+///
+/// The hash state is kept in an accumulator, with
+/// - an initial value
+/// - an update function, adding a block of bytes;
+/// - an extract function, returning a hash tag.
+///
+/// Before hashing, some algorithm-specific padding and length
+/// encoding is appended to the input bytestring.
+///
+/// This is not a general-purpose incremental specification, which
+/// would support adding text fragments of arbitrary lengths.
+
+//18-07-06 switching to ghosts for uniformity, but not great at the pure code actually works concretely.
+//18-07-06 a better name than repr_t?
+noextract val acc (a: e_alg): Type0 // noeq, but `noeq val` is not supported)
+
+(* sets the initial value of the accumulator *) 
+noextract val acc0 (#a:e_alg): GTot (acc a)
+
+(* hashes one block of data into the accumulator *)
+noextract val compress: #a:e_alg -> acc a -> b: lbytes (blockLength a) -> GTot (acc a)
+
+(* extracts the tag from the (possibly larger) accumulator *)
+noextract val extract: #a:e_alg -> acc a -> lbytes (tagLength a)
+ 
+// val hash2: #a:alg -> acc a -> b:bytes {length b % blockLength a = 0} -> acc a (decreases (length b))
+noextract let rec hash2 
+  (#a:e_alg) 
+  (v:acc a) 
+  (b:bytes {Seq.length b % blockLength a = 0}): 
+  GTot (acc a) (decreases (Seq.length b))
+=  
+  if Seq.length b = 0 then v
+  else
+    let c,b = Seq.split b (blockLength a) in
+    hash2 (compress v c) b
+
+let lemma_compress 
+  (#a: e_alg) 
+  (a0: acc a)
+  (c: lbytes (blockLength a)): 
+  Lemma (compress a0 c == hash2 a0 c) = ()
+
+let rec lemma_hash2 
+  (#a: e_alg) 
+  (a0: acc a)
+  (b0 b1: (b:bytes{ Seq.length b % blockLength a = 0})): 
+  Lemma 
+    (ensures hash2 a0 (Seq.append b0 b1) == hash2 (hash2 a0 b0) b1)
+    (decreases (Seq.length b0)) 
+=
+  if Seq.length b0 = 0 then (
+    Seq.lemma_empty b0;
+    Seq.append_empty_l b1 )
+  else (
+    let c,b0' = Seq.split b0 (blockLength a) in
+    let c',b' = Seq.split (Seq.append b0 b1) (blockLength a) in
+    Seq.append_assoc c b0' b1;
+    //Seq.lemma_split b0 (blockLength a);
+    //Seq.lemma_eq_intro (Seq.append b0 b1) (Seq.append c' b');
+    Seq.lemma_eq_intro c c';
+    Seq.lemma_eq_intro b' (Seq.append b0' b1);
+    lemma_hash2 (hash2 a0 c) b0' b1)
+
+noextract let hash0 (#a:e_alg) (b:bytes {Seq.length b % blockLength a = 0}) = hash2 (acc0 #a) b
+
+/// PADDING AND LENGTH ENCODING
+/// for convenience, we treat inputs as sequences of bytes, not bits.
+/// but note that the suffix encodes the length in bits.
+private noextract
+let suffixLength (a:e_alg) (length:nat {length <= maxLength a}): 
+  GTot (n:nat{ (length + n) % blockLength a = 0 /\ n <= blockLength a + 9 })
+=
+  let blocklen = blockLength a in 
+  let lenlen = match Ghost.reveal a with | SHA384 | SHA512 -> 8 | _ -> 4 in
+  let required =  length + 1 + lenlen in // minimal length after padding and encoding the length
+  let zeros = // minimal extra padding for block alignment
+    if required % blocklen = 0 
+    then 0
+    else blocklen - (required % blocklen) in
+    //was, harder to prove: required + blockLen a - ((required - 1) % blockLen a + 1) in
+  1 + zeros + lenlen
+
+noextract val suffix: a:e_alg -> l:nat {l <= maxLength a} -> GTot (lbytes (suffixLength a l))
+
+// would prefer to name it [hash] but already taken below
+noextract let spec (a:e_alg) (b:hashable a): GTot (lbytes (tagLength a)) =
+  let blocks = Seq.append b (suffix a (Seq.length b)) in
+  let acc = hash0 blocks in
+  let tag = extract acc in
+  tag
+
+// TODO most users of the spec would prefer a more opaque specification
+// can we use [abstract] or something similar to hide the structure?
+
+
+/// 18-04-07 postponing verified integration with HACL* for now. We
+/// provide below a concise definition of the Merkle-Damgard
+/// construction. The plan is to integrate it with Benjamin's
+/// algorithmic specifications. At that point, we will probably hide
+/// the construction behind the provider interface (since we don't
+/// care about the construction when using or reasoning about them).
+
+/// 
+/// ----------agile interface to hash specifications ----------------
+
+
+
+
 
 module HS = FStar.HyperStack
 module B = LowStar.Buffer
@@ -12,15 +194,8 @@ module G = FStar.Ghost
 open LowStar.BufferOps
 
 let uint8_p = B.buffer UInt8.t
-let bytes = Seq.seq UInt8.t
 
-type alg =
-| SHA256
-| SHA384
-
-type e_alg =
-  G.erased alg
-
+// abstract implementation state
 val state_s: e_alg -> Type0
 let state alg = B.pointer (state_s alg)
 
@@ -36,24 +211,9 @@ let invariant (#a: e_alg) (s: state a) (m: HS.mem) =
   M.(loc_disjoint (loc_buffer s) (footprint_s (deref m s))) /\
   invariant_s (B.get m s 0) m
 
-let type_of alg =
-  match G.reveal alg with
-  | SHA256 -> uint_32
-  | SHA384 -> uint_64
-
-let size_of_k alg =
-  match G.reveal alg with
-  | SHA256 -> 64
-  | SHA384 -> 80
-
-type repr_t (a: e_alg) = {
-  k: Seq.lseq (type_of a) (size_of_k a);
-  hash: Seq.lseq (type_of a) 8;
-  counter: nat;
-}
-
+//18-07-06 as_acc a better name? not really a representation
 val repr: #a:e_alg -> s:state a -> h:HS.mem { invariant s h } ->
-  GTot (repr_t a)
+  GTot (acc a)
 
 // Waiting for these to land in LowStar.Modifies
 let loc_in (l: M.loc) (h: HS.mem) =
@@ -99,56 +259,24 @@ val create: a:alg -> ST (state (G.hide a))
     M.(modifies loc_none h0 h1) /\
     fresh_loc (footprint s h1) h0 h1)
 
-let init_repr (a: e_alg): GTot (repr_t a) =
-  match G.reveal a with
-  | SHA256 -> {
-      hash = EverCrypt.Spec.SHA2_256.h_0;
-      k = EverCrypt.Spec.SHA2_256.k;
-      counter = 0
-    }
-  | SHA384 -> {
-      hash = EverCrypt.Spec.SHA2_384.h_0;
-      k = EverCrypt.Spec.SHA2_384.k;
-      counter = 0
-    }
-
 val init: #a:e_alg -> s:state a -> ST unit
   (requires (invariant s))
   (ensures (fun h0 _ h1 ->
     invariant s h1 /\
     M.(modifies (footprint s h0) h0 h1) /\
     footprint s h0 == footprint s h1 /\
-    repr s h1 == init_repr a))
+    repr s h1 == acc0 #a))
 
-let block_size a: GTot _ =
-  match G.reveal a with
-  | SHA256 -> EverCrypt.Spec.SHA2_256.size_block
-  | SHA384 -> EverCrypt.Spec.SHA2_384.size_block
+val well_formed: 
+  #a:e_alg -> 
+  s: state a ->
+  h: HS.mem{invariant s h} -> GTot Type0
 
-let well_formed (#a:e_alg)
-  (s: state a)
-  (h: HS.mem{invariant s h}):
-  GTot _
-=
-  let r = repr s h in
-  match G.reveal a with
-  | SHA256 ->
-      r.k == EverCrypt.Spec.SHA2_256.k
-  | SHA384 ->
-      r.k == EverCrypt.Spec.SHA2_384.k
-
-let bounded_counter (#a:e_alg)
-  (s: state a)
-  (h: HS.mem{invariant s h})
-  (n: nat { n <= pow2 32 }):
-  GTot _
-=
-  let r = repr s h in
-  match G.reveal a with
-  | SHA256 ->
-      r.counter < pow2 32 - n
-  | SHA384 ->
-      r.counter < pow2 32 - n
+val bounded_counter:
+  #a:e_alg ->
+  s: state a ->
+  h: HS.mem{invariant s h} ->
+  n: nat { n <= pow2 32 } -> GTot Type0
 
 let well_formed_and_counter (#a:e_alg)
   (s: state a)
@@ -157,21 +285,6 @@ let well_formed_and_counter (#a:e_alg)
   GTot _
 =
   well_formed s h /\ bounded_counter s h n
-
-let update_spec (#a:e_alg)
-  (s:state a)
-  (h0: HS.mem{invariant s h0})
-  (h1: HS.mem{invariant s h1})
-  (data: bytes{Seq.length data = block_size a}):
-  GTot _
-=
-  let r0 = repr s h0 in
-  let r1 = repr s h1 in
-  match G.reveal a with
-  | SHA256 ->
-      r1.hash = EverCrypt.Spec.SHA2_256.update r0.hash data
-  | SHA384 ->
-      r1.hash = EverCrypt.Spec.SHA2_384.update r0.hash data
 
 // Note: this function relies implicitly on the fact that we are running with
 // code/lib/kremlin and that we know that machine integers and secret integers
@@ -182,44 +295,35 @@ val update: #a:e_alg -> s:state a -> data:uint8_p -> Stack unit
     invariant s h0 /\
     well_formed_and_counter s h0 1 /\
     B.live h0 data /\
-    B.length data = block_size a /\
+    B.length data = blockLength a /\
     M.(loc_disjoint (footprint s h0) (loc_buffer data))))
   (ensures (fun h0 _ h1 ->
     invariant s h1 /\
     M.(modifies (footprint s h0) h0 h1) /\
     footprint s h0 == footprint s h1 /\
-    well_formed_and_counter s h1 0 /\
-    update_spec s h0 h1 (B.as_seq h0 data)))
-
-let update_multi_spec (#a:e_alg)
-  (s:state a)
-  (h0: HS.mem{invariant s h0})
-  (h1: HS.mem{invariant s h1})
-  (data: bytes{Seq.length data % block_size a = 0}):
-  GTot _
-=
-  let r0 = repr s h0 in
-  let r1 = repr s h1 in
-  match G.reveal a with
-  | SHA256 ->
-      r1.hash = EverCrypt.Spec.SHA2_256.update_multi r0.hash data
-  | SHA384 ->
-      r1.hash = EverCrypt.Spec.SHA2_384.update_multi r0.hash data
+    well_formed_and_counter s h1 0 /\ (
+    let r0 = repr s h0 in
+    let r1 = repr s h1 in
+    r1 == compress r0 (B.as_seq h0 data))))
 
 val update_multi: #a:e_alg -> s:state a -> data:uint8_p -> n:UInt32.t -> Stack unit
   (requires (fun h0 ->
     invariant s h0 /\
     well_formed_and_counter s h0 (v n) /\
     B.live h0 data /\
-    B.length data = block_size a * v n /\
+    B.length data = blockLength a * v n /\
     M.(loc_disjoint (footprint s h0) (loc_buffer data))))
   (ensures (fun h0 _ h1 ->
     invariant s h1 /\
     M.(modifies (footprint s h0) h0 h1) /\
     footprint s h0 == footprint s h1 /\
-    well_formed_and_counter s h1 0 /\
-    update_multi_spec s h0 h1 (B.as_seq h0 data)))
+    well_formed_and_counter s h1 0 /\ (
+    let r0 = repr s h0 in 
+    let r1 = repr s h1 in
+    r1 == hash2 r0 (B.as_seq h0 data))))
 
+
+(* see suffix and suffixLength 
 // The maximum number of bytes for the input.
 let max_input_length (a: e_alg): GTot _ =
   match G.reveal a with
@@ -231,27 +335,30 @@ let max_input_length (a: e_alg): GTot _ =
 // The size, in bytes, it takes to encode the number of bytes in the message.
 let size_length (a: e_alg): GTot _ =
   match G.reveal a with
-  | SHA256 ->
-      EverCrypt.Spec.SHA2_256.size_len_8
-  | SHA384 ->
-      EverCrypt.Spec.SHA2_384.size_len_8
+  | SHA384 | SHA512 -> 8 
+  | _               -> 4
 
 // For the last (possibly partial) block, in so far as I understand, we
 // concatenate the last chunk of data, insert a byte 0x01, then encode the length.
 let last_data_fits (a: e_alg) (length: nat): GTot _ =
   length + size_length a + 1 < 2 * block_size a
+*) 
 
+(*
 // Note: conjunction of well_formed and last_data_fits allows deriving the
 // specific precondition for update_last.
 let update_last_spec (#a:e_alg)
   (s:state a)
   (h0: HS.mem{invariant s h0})
   (h1: HS.mem{invariant s h1})
-  (data: bytes{well_formed_and_counter s h0 2 /\ last_data_fits a (Seq.length data)}):
+  (data: bytes{
+    well_formed_and_counter s h0 2 /\ 
+    last_data_fits a (Seq.length data)}):
   GTot _
 =
   let r0 = repr s h0 in
   let r1 = repr s h1 in
+  
   let counter0 = r0.counter in
   let len0 = counter0 * block_size a in
   match G.reveal a with
@@ -259,68 +366,59 @@ let update_last_spec (#a:e_alg)
       r1.hash = EverCrypt.Spec.SHA2_256.update_last r0.hash len0 data
   | SHA384 ->
       r1.hash = EverCrypt.Spec.SHA2_384.update_last r0.hash len0 data
+*)
 
-val update_last: #a:e_alg -> s:state a -> data:uint8_p -> len:UInt32.t -> Stack unit
+// 18-03-05 note the *new length-passing convention!
+// 18-03-03 it is best to let the caller keep track of lengths.
+// 18-03-03 the last block is *never* complete so there is room for the 1st byte of padding.
+val update_last: 
+  #a:e_alg -> 
+  s:state a -> 
+  last:uint8_p {
+    B.length last <= blockLength a } -> 
+  total_len:UInt32.t {
+    let l = v total_len in 
+    l <= maxLength a /\
+    B.length last = l % blockLength a } -> Stack unit
   (requires (fun h0 ->
     invariant s h0 /\
     well_formed_and_counter s h0 2 /\
-    B.live h0 data /\
-    B.length data = v len /\
-    last_data_fits a (v len) /\
-    M.(loc_disjoint (footprint s h0) (loc_buffer data))))
+    B.live h0 last /\
+    M.(loc_disjoint (footprint s h0) (loc_buffer last))))
   (ensures (fun h0 _ h1 ->
     invariant s h1 /\
     M.(modifies (footprint s h0) h0 h1) /\
     footprint s h0 == footprint s h1 /\
-    well_formed s h1 /\
-    update_last_spec s h0 h1 (B.as_seq h0 data)))
-
-let hash_size a: GTot _ =
-  match G.reveal a with
-  | SHA256 -> EverCrypt.Spec.SHA2_256.size_hash
-  | SHA384 -> EverCrypt.Spec.SHA2_384.size_hash
-
-let finish_spec (#a:e_alg)
-  (s:state a)
-  (h0: HS.mem{invariant s h0})
-  (dst: bytes{Seq.length dst = hash_size a}):
-  GTot _
-=
-  let r0 = repr s h0 in
-  match G.reveal a with
-  | SHA256 ->
-      dst = EverCrypt.Spec.SHA2_256.finish r0.hash
-  | SHA384 ->
-      dst = EverCrypt.Spec.SHA2_384.finish r0.hash
+    well_formed s h1 /\ (
+    let r0 = repr s h0 in
+    let r1 = repr s h1 in
+    let last0 = B.as_seq h0 last in 
+    let rawbytes = Seq.append last0 (suffix a (v total_len)) in
+    Seq.length rawbytes % blockLength a = 0 (*required by hash2; otherwise brittle*) /\ 
+    r1 == hash2 #a r0 rawbytes)))
 
 val finish: #a:e_alg -> s:state a -> dst:uint8_p -> Stack unit
   (requires (fun h0 ->
     invariant s h0 /\
     well_formed s h0 /\
     B.live h0 dst /\
-    B.length dst = hash_size a /\
+    B.length dst = tagLength a /\
     M.(loc_disjoint (footprint s h0) (loc_buffer dst))))
   (ensures (fun h0 _ h1 ->
     invariant s h1 /\
     M.(modifies (loc_buffer dst) h0 h1) /\
-    footprint s h0 == footprint s h1 /\
-    finish_spec s h0 (B.as_seq h1 dst)))
-
-let hash_spec (a: alg) (input: bytes{Seq.length input < max_input_length (G.hide a)}): GTot _ =
-  match a with
-  | SHA256 ->
-      EverCrypt.Spec.SHA2_256.hash input
-  | SHA384 ->
-      EverCrypt.Spec.SHA2_384.hash input
+    footprint s h0 == footprint s h1 /\ 
+    B.as_seq h1 dst = extract (repr s h0)))
 
 val hash: a:alg -> dst:uint8_p -> input:uint8_p -> len:uint32_t -> Stack unit
   (requires (fun h0 ->
+    let a = Ghost.hide a in 
     B.live h0 dst /\
     B.live h0 input /\
     B.length input = v len /\
-    v len < max_input_length (G.hide a) /\
-    B.length dst = hash_size (G.hide a) /\
+    v len < maxLength a /\
+    B.length dst = tagLength a /\
     M.(loc_disjoint (loc_buffer input) (loc_buffer dst))))
   (ensures (fun h0 _ h1 ->
     M.(modifies (loc_buffer dst) h0 h1) /\
-    B.as_seq h1 dst = hash_spec a (B.as_seq h0 input)))
+    B.as_seq h1 dst = spec (Ghost.hide a) (B.as_seq h0 input)))
