providers/evercrypt/fst/EverCrypt.Hash.fst
@@ -1,5 +1,143 @@
 module EverCrypt.Hash
 
+/// ----------agile implementation of hash specification ------------
+/// must be in scope for linking the agile spec to the ad hoc algorithmic specs
+
+let string_of_alg = function
+  | MD5    -> "MD5"
+  | SHA1   -> "SHA1"
+  | SHA224 -> "SHA224"
+  | SHA256 -> "SHA256"
+  | SHA384 -> "SHA384"
+  | SHA512 -> "SHA512"
+
+
+let type_of a =
+  match Ghost.reveal a with
+  | MD5 | SHA1 | SHA224 | SHA256 -> UInt32.t // uint_32
+  | SHA384 | SHA512              -> UInt64.t // uint_64
+
+let size_of_k a: GTot nat =
+  match Ghost.reveal a with
+  | SHA256 -> 64
+  | SHA384 -> 80
+  | _      -> admit()
+
+type acc (a: e_alg) = {
+  k: Seq.lseq (type_of a) (size_of_k a);
+  hash: Seq.lseq (type_of a) 8;
+  counter: nat;
+}
+
+let acc0 #a =
+  match Ghost.reveal a with
+  | SHA256 -> {
+      hash = EverCrypt.Spec.SHA2_256.h_0;
+      k = EverCrypt.Spec.SHA2_256.k;
+      counter = 0
+    }
+  | SHA384 -> {
+      hash = EverCrypt.Spec.SHA2_384.h_0;
+      k = EverCrypt.Spec.SHA2_384.k;
+      counter = 0
+    }
+  | _ -> admit()
+
+// 18-07-06 We need a fully-specified refinement: the hacl* spec
+// should state that the counter is incremented by 1 and that the K
+// constant is unchanged---a total spec would also save the need for
+// stateful invariants.
+//
+// Besides, all of that could be avoided if the state was just the
+// intermediate hash.
+
+let compress #a st b = 
+  match Ghost.reveal a with 
+  | SHA256 -> 
+     { k       = EverCrypt.Spec.SHA2_256.k; 
+       hash    = EverCrypt.Spec.SHA2_256.update st.hash b;
+       counter = st.counter + 1 } 
+  | SHA384 -> 
+     { k       = EverCrypt.Spec.SHA2_384.k; 
+       hash    = EverCrypt.Spec.SHA2_384.update st.hash b;
+       counter = st.counter + 1 } 
+  | _ -> 
+    admit()
+  
+(* was, partial:
+let update_spec (#a:e_alg)
+  (s:state a)
+  (h0: HS.mem{invariant s h0})
+  (h1: HS.mem{invariant s h1})
+  (data: bytes{Seq.length data = block_size a}):
+  GTot _
+=
+  let r0 = repr s h0 in
+  let r1 = repr s h1 in
+  match G.reveal a with
+  | SHA256 -> r1.hash = EverCrypt.Spec.SHA2_256.update r0.hash data
+  | SHA384 -> r1.hash = EverCrypt.Spec.SHA2_384.update r0.hash data
+*)
+
+// 18-07-06 hacl* defines finish on the raw buffer contents, so
+// we'd need to define repr first.
+let extract #a st = admit()
+(*
+  match Ghost.reveal a with 
+  | SHA256 -> repr Spec.SHA2_256.finish st 
+  | SHA384 -> Spec.SHA2_384.finish st 
+  | _ -> admit()
+*)
+
+// 18-07-06 should be provable, despite the two specs having different
+// structures.
+let suffix a l = admit()
+(*
+  let l1 = l % blockLength a in 
+  let l0 = l - l1 in
+  match Ghost.reveal a with
+  | SHA256 -> 
+      assume(l0 % blockLength a == 0);
+      assume(l < Spec.SHA2_256.max_input_len_8); 
+      let pad = Spec.SHA2_256.pad l0 l1 in
+      assume(Seq.length pad = suffixLength a l);
+      pad
+  | _ -> admit()
+//| SHA384 -> Spec.SHA2_384.pad l0 l1 
+//| SHA512 -> Spec.SHA2_512.pad l0 l1
+*)
+
+
+(*
+  match G.reveal a with
+  | SHA256 ->
+      r1.hash = EverCrypt.Spec.SHA2_256.update r0.hash data
+  | SHA384 ->
+      r1.hash = EverCrypt.Spec.SHA2_384.update r0.hash data
+
+// from update_multi_spec: 
+  match G.reveal a with
+  | SHA256 ->
+      r1.hash = EverCrypt.Spec.SHA2_256.update_multi r0.hash data
+  | SHA384 ->
+      r1.hash = EverCrypt.Spec.SHA2_384.update_multi r0.hash data
+*)
+
+/// 18-04-07 postponing verified integration with HACL* for now. We
+/// provide below a concise definition of the Merkle-Damgard
+/// construction. The plan is to integrate it with Benjamin's
+/// algorithmic specifications. At that point, we will probably hide
+/// the construction behind the provider interface (since we don't
+/// care about the construction when using or reasoning about them).
+
+
+/// 
+/// ----------agile implementation of hash specification ------------
+
+
+
+
+
 open FStar.HyperStack.ST
 
 module U32  = FStar.UInt32
@@ -38,12 +176,9 @@ let footprint_s #a (s: state_s a): GTot M.loc =
 
 let invariant_s #a s h =
   match s with
-  | SHA256_Hacl p ->
-      B.live h p
-  | SHA256_Vale p ->
-      B.live h p
-  | SHA384_Hacl p ->
-      B.live h p
+  | SHA256_Hacl p -> B.live h p
+  | SHA256_Vale p -> B.live h p
+  | SHA384_Hacl p -> B.live h p
 
 let repr #a s h: GTot _ =
   let s = B.get h s 0 in
@@ -68,8 +203,9 @@ let repr #a s h: GTot _ =
         hash = Hacl.SHA2_384.slice_hash h p;
         counter = Hacl.SHA2_384.counter h p
       }
+  | _ -> admit()
 
-let repr_eq (#a:e_alg) (r1 r2: repr_t a) =
+let repr_eq (#a:e_alg) (r1 r2: acc a) =
   Seq.equal r1.k r2.k /\
   Seq.equal r1.hash r2.hash /\
   r1.counter = r2.counter
@@ -122,6 +258,31 @@ let init #a s =
       admit ()
 
 #set-options "--z3rlimit 20"
+
+
+let well_formed (#a:e_alg)
+  (s: state a)
+  (h: HS.mem{invariant s h}):
+  GTot _
+=
+  let r = repr s h in
+  match G.reveal a with
+  | SHA256 -> r.k == EverCrypt.Spec.SHA2_256.k
+  | SHA384 -> r.k == EverCrypt.Spec.SHA2_384.k
+  | _ -> admit()
+
+let bounded_counter (#a:e_alg)
+  (s: state a)
+  (h: HS.mem{invariant s h})
+  (n: nat { n <= pow2 32 }):
+  GTot _
+=
+  let r = repr s h in
+  match G.reveal a with
+  | SHA256 -> r.counter < pow2 32 - n
+  | SHA384 -> r.counter < pow2 32 - n
+  | _ -> admit()
+
 
 let update #a s data =
   match !*s with
